ThoR/Semantics/Semantics.lean
@@ -9,7 +9,7 @@ import ThoR.Relation.Quantification
 import ThoR.Relation.Rel
 -- import ThoR.Relation.Elab
 
-import ThoR.Semantics.RelList
+import ThoR.Semantics.HList
 
 namespace ThoR.Semantics
 
@@ -26,43 +26,86 @@ variable (R : Type) [TupleSet R]
 
   -- abbrev RelFunc (R : Type) [TupleSet R] {return_type : Type w}:= @HFunc _ (λ (type : RelTypeWithArity R) => Rel type.2) return_type
 
+-- construction follows https://lean-lang.org/documentation/examples/debruijn/
 
-  inductive SemType {R : Type} [TupleSet R] : Type u where
+
+  inductive Ty {R : Type} [TupleSet R] : Type u where
     | number -- ℤ
     | formula -- Prop
-    | expression : {n : ℕ} → (rel_type : RelType R n) → SemType -- Rel rel_type
-    | expression_list : (indices : List (RelTypeWithArity R)) → SemType -- RelList indices
-    | function : SemType → SemType → SemType -- st1.eval → st2.eval
+    | expression : {n : ℕ} → (rel_type : RelType R n) → Ty -- Rel rel_type
+--    | expression_list : (indices : List (RelTypeWithArity R)) → Ty -- RelList indices
+    | function : Ty → Ty → Ty -- st1.eval → st2.eval
 
-  inductive Term {R : Type} [TupleSet R] : @SemType R _ → Type u where
-    | rel {n : ℕ} {t : RelType R n} (r : Rel t) : Term (.expression t)
+  @[reducible]
+  def Ty.eval {R : Type} [TupleSet R] (ty : @Ty R _) :=
+    match ty with
+    | number => ℤ
+    | formula => Prop
+    | expression rel_type => Rel rel_type
+    | function dom ran => dom.eval → ran.eval
 
-    | intersect {n : ℕ} {t1 t2 : RelType R n} : Term (.expression t1) → Term (.expression t2)  → Term (.expression (t1 & t2))
-    | transclos {t : RelType R 2} : Term (.expression t) → Term (.expression (^ t))
+  inductive Term {R : Type} [TupleSet R] : List (@Ty R _) → (@Ty R _) → Type u where
+    | rel {n : ℕ} {t : RelType R n} (r : Rel t) : Term ctx (.expression t)
 
-    | if_then_else {n : ℕ} {t1 t2 : RelType R n} : Term .formula → Term (.expression t1) → Term (.expression t2) → Term (.expression (RelType.ifThenElse t1 t2))
+    | var : (ty : @Ty R _) → Member ty ctx → Term ctx ty
 
-    | pred {n : ℕ} {t : RelType R n} : (Rel t → Term .formula) → Term (.function (.expression_list indices) .formula)
+    | intersect {n : ℕ} {t1 t2 : RelType R n} : Term ctx (.expression t1) → Term ctx (.expression t2)  → Term ctx (.expression (t1 & t2))
+    | transclos {t : RelType R 2} : Term ctx (.expression t) → Term ctx (.expression (^ t))
 
-    | pred_application {indices : List (RelTypeWithArity R)} : Term (.function (.expression_list indices) .formula) → RelList R indices → Term .formula
+    | if_then_else {n : ℕ} {t1 t2 : RelType R n} : Term ctx .formula → Term ctx (.expression t1) → Term ctx (.expression t2) → Term ctx (.expression (RelType.ifThenElse t1 t2))
 
-    | number (z : ℤ) : Term .number
-    | negation : Term .number → Term .number
-    | add : Term .number → Term .number → Term .number
-    | card {n : ℕ} {t : RelType R n} : Term (.expression t) → Term .number
+    | app   : Term ctx (.function dom ran) → Term ctx dom → Term ctx ran
+    | lam   : Term (dom :: ctx) ran → Term ctx (.function dom ran)
 
-    | lone {n : ℕ} {t : RelType R n} : Term (.expression t) → Term .formula
+    | number (z : ℤ) : Term ctx .number
+    | negation : Term ctx .number → Term ctx .number
+    | add : Term ctx .number → Term ctx .number → Term ctx .number
+    | card {n : ℕ} {t : RelType R n} : Term ctx (.expression t) → Term ctx .number
 
-    | not : Term .formula → Term .formula
-    | or : Term .formula → Term .formula → Term .formula
+    | lone {n : ℕ} {t : RelType R n} : Term ctx (.expression t) → Term ctx .formula
 
-    | f_if_then_else : Term .formula → Term .formula → Term .formula → Term .formula
+    | not : Term ctx .formula → Term ctx .formula
+    | or : Term ctx .formula → Term ctx .formula → Term ctx .formula
 
-    | a_lt : Term .number → Term .number → Term .formula
+    | f_if_then_else : Term ctx .formula → Term ctx .formula → Term ctx .formula → Term ctx .formula
 
-    | in {n : ℕ} {t1 t2 : RelType R n} : Term (.expression t1) → Term (.expression t2) → Term .formula
+    | a_lt : Term ctx .number → Term ctx .number → Term ctx .formula
 
-    | q_all {n : ℕ} {t : RelType R n} : Term (.function (.expression t) ran) → Term .formula -- (f : (Rel t) → Formula): Formula
+    | in {n : ℕ} {t1 t2 : RelType R n} : Term ctx (.expression t1) → Term ctx (.expression t2) → Term ctx .formula
+
+    -- | q_all {n : ℕ} {t : RelType R n} : Term ctx (.function (.expression t) ran) → Term ctx .formula -- (f : (Rel t) → Formula): Formula
+
+  def Term.eval {R : Type} [TupleSet R] {ctx: List (@Ty R _)} {ty : @Ty R _} (t : @Term R _ ctx ty) (env : HList Ty.eval ctx): ty.eval :=
+    match t with
+    | .rel r => r
+
+    | .var t h => env.get h
+
+    | .intersect r1 r2 => (r1.eval env) & (r2.eval env)
+    | .transclos r => ^ (r.eval env)
+    | .if_then_else f r1 r2 => HIfThenElse.hIfThenElse (f.eval env) (r1.eval env) (r2.eval env)
+
+    | .lam b => λ x => b.eval (x :: env)
+    | .app f a => f.eval env (a.eval env)
+
+    | .number z => z
+    | .negation z => - (z.eval env)
+    | .add z1 z2 => (z1.eval env) + (z2.eval env)
+    | .card r => Card.card (r.eval env)
+
+    | .lone r => SetMultPredicates.lone (r.eval env)
+
+    | .not f => ¬ (f.eval env)
+    | .or f1 f2 => (f1.eval env) ∨ (f2.eval env)
+
+    | .f_if_then_else f1 f2 f3 =>
+      ((f1.eval env) -> (f2.eval env)) ∧ (¬ (f1.eval env) → (f2.eval env))
+
+    | .a_lt z1 z2 => (z1.eval env) < (z2.eval env)
+
+    | .in r1 r2 => (r1.eval env) ⊂ (r2.eval env)
+
+    -- | q_all {n : ℕ} {t : RelType R n} : Term ctx (.function (.expression t) ran) → Term ctx .formula -- (f : (Rel t) → Formula): Formula
 
 end ThoR.Semantics
 
@@ -74,83 +117,41 @@ class vars (R : Type) [TupleSet R] where
 
 variable (ThoR_TupleSet : Type) [TupleSet ThoR_TupleSet] [vars ThoR_TupleSet]
 
--- @[default_instance]
--- instance : ThoR.TupleSet ThoR_TupleSet := by sorry
+-- pred_in1 [x : set univ] {
+--    x in x
+-- }
+#check (Term.var (Ty.expression (RelType.mk.sig ThoR_TupleSet Shared.mult.set)) (Member.head))
+#check (Term.in (Term.var (Ty.expression (RelType.mk.sig ThoR_TupleSet Shared.mult.set)) (Member.head)) (Term.var (Ty.expression (RelType.mk.sig ThoR_TupleSet Shared.mult.set)) (Member.head)))
 
--- @[default_instance]
--- instance : vars ThoR_TupleSet := by sorry
+#check Term.lam (Term.in (Term.var (Ty.expression (RelType.mk.sig ThoR_TupleSet Shared.mult.set)) (Member.head)) (Term.var (Ty.expression (RelType.mk.sig ThoR_TupleSet Shared.mult.set)) (Member.head)))
 
+def pred_in1 := @Term.lam ThoR_TupleSet _ _ [] (Term.in (Term.var (Ty.expression (RelType.mk.sig ThoR_TupleSet Shared.mult.set)) (Member.head)) (Term.var (Ty.expression (RelType.mk.sig ThoR_TupleSet Shared.mult.set)) (Member.head)))
 
-def u := Term.rel (@vars.UNIV ThoR_TupleSet _ _)
-#check u
+#print pred_in1
 
-#check Term.in (@u ThoR_TupleSet _ _) (@u ThoR_TupleSet _ _)
+-- pred_in2 [x : set univ] {
+--    x in univ
+-- }
+def pred_in2 := @Term.lam _ _ _ [] (Term.in (Term.var (Ty.expression (RelType.mk.sig ThoR_TupleSet Shared.mult.set)) (Member.head)) (Term.rel (@vars.UNIV ThoR_TupleSet _ _)))
 
+example : (Term.pred_app (@pred_in1 ThoR_TupleSet _) (Term.rel (@vars.UNIV ThoR_TupleSet _ _))).eval [] := by
+  simp [Term.eval]
+  simp [HList.get]
+  apply Set.subset_refl
 
-#check @HFunc.const  _ _ (RelType ThoR_TupleSet) (Term.in (@u ThoR_TupleSet _ _) (@u ThoR_TupleSet _ _))
+example : (Term.pred_app (@pred_in2 ThoR_TupleSet _ _) (Term.rel (@vars.UNIV ThoR_TupleSet _ _))).eval [] := by
+  simp [Term.eval]
+  simp [HList.get]
+  apply Set.subset_refl
 
-#check HFunc.abstraction (
-    λ (r3 : Rel (RelType.mk.sig ThoR_TupleSet Shared.mult.set)) =>
-      HFunc.const (
-        (Term.in (Term.rel r3) (Term.rel r3))
-      )
-  )
-
+-- pred_in3 [x : set univ, y : set univ] {
+--    x in y
+-- }
 #check
-  HFunc.abstraction (
-    λ (r2 : Rel (RelType.mk.sig ThoR_TupleSet Shared.mult.set)) =>
-      HFunc.abstraction (
-        λ (r3 : Rel (RelType.mk.sig ThoR_TupleSet Shared.mult.set)) =>
-          HFunc.const (
-            (Term.in (Term.rel r2) (Term.rel r3))
-          )
-      )
+  Term.lam (
+    Term.lam (
+      Term.in
+        (Term.var (Ty.expression (RelType.mk.sig ThoR_TupleSet Shared.mult.set)) (Member.head))
+        (Term.rel (@vars.UNIV ThoR_TupleSet _ _))
+    )
   )
-
-#check
-  HFunc.abstraction (
-    λ (r1 : Rel (RelType.mk.sig ThoR_TupleSet Shared.mult.set)) =>
-      HFunc.abstraction (
-        λ (r2 : Rel (RelType.mk.sig ThoR_TupleSet Shared.mult.set)) =>
-          HFunc.abstraction (
-            λ (r3 : Rel (RelType.mk.sig ThoR_TupleSet Shared.mult.set)) =>
-              HFunc.const (
-                Term.or (Term.in (Term.rel r1) (Term.rel r2)) (Term.in (Term.rel r2) (Term.rel r3))
-              )
-          )
-      )
-  )
-
-
-
-def pred3 :=
-  HFunc.abstraction (
-    λ (r1 : Rel (RelType.mk.sig ThoR_TupleSet Shared.mult.set)) =>
-      HFunc.abstraction (
-        λ (r2 : Rel (RelType.mk.sig ThoR_TupleSet Shared.mult.set)) =>
-          HFunc.abstraction (
-            λ (r3 : Rel (RelType.mk.sig ThoR_TupleSet Shared.mult.set)) =>
-              HFunc.const (
-                Term.or (Term.in (Term.rel r1) (Term.rel r2)) (Term.in (Term.rel r2) (Term.rel r3))
-              )
-          )
-      )
-  )
-
-#check RelType'
-#print pred3
-
-
-
-  -- inductive HFunc {α : Type v} (β : α → Type u) (return_type : Type w): List α → Type (max u v w) where
-  --   | const : return_type → HFunc β return_type []
-  --   | abstraction : (β i → HFunc β return_type is) → HFunc β return_type (i::is)
-  --   | application : β i → HFunc β return_type (i::is) → HFunc β return_type is
-
-#check pred3 _
-#check
-  HFunc.application (
-    HFunc.application (
-      HFunc.application (pred3 ThoR_TupleSet) (@vars.UNIV ThoR_TupleSet _ _)
-    ) (@vars.UNIV ThoR_TupleSet _ _)
-  ) (@vars.UNIV ThoR_TupleSet _ _)
